Delete more unnecessary stuff; prove some wp_load/store instances

new/golang/theory/intoval.v
@@ -7,6 +7,9 @@ From Ltac2 Require Import Ltac2.
 Set Default Proof Mode "Classic".
 From New.golang.defn Require Export postlang.
 
+Section defs.
+(** Proven (i.e. untrusted) definitions and properties associated with types `V`
+    that have an `IntoVal` instance. *)
 Class IntoValProof (V : Type) `{IntoVal V} :=
   {
     typed_pointsto_def `{sem: ffi_semantics} `{!ffi_interp ffi} `{!heapGS Σ}
@@ -21,9 +24,13 @@ Notation "l ↦ dq v" := (typed_pointsto l dq v%V)
                          (at level 20, dq custom dfrac at level 1,
                             format "l  ↦ dq  v") : bi_scope.
 
-Section defs.
 Context `{sem: ffi_semantics} `{!ffi_interp ffi} `{!heapGS Σ}.
-Context `{!NamedUnderlyingTypes}.
+(** [IntoValTyped V t] provides proofs that loading and storing [t] respects
+    the typed points-to for `V`.
+
+    [typed_pointsto_def] is in [IntoValProof] rather than here because `l ↦ v`
+    not explicitly mention `t`, and there can be multiple `t`s for a single `V`
+    (e.g. int64 and uint64 both have w64). *)
 Class IntoValTyped (V : Type) (t : go.type) `{!IntoVal V} `{!IntoValProof V} :=
   {
     wp_load : (∀ l dq (v : V), {{{ l ↦{dq} v }}}
@@ -31,8 +38,8 @@ Class IntoValTyped (V : Type) (t : go.type) `{!IntoVal V} `{!IntoValProof V} :=
                                {{{ RET #v; l ↦{dq} v }}});
     wp_store : (∀ l (v w : V), {{{ l ↦ v }}}
                                  store t #l #w
-                               {{{ RET #v; l ↦ w }}});
+                               {{{ RET #(); l ↦ w }}});
   }.
-(* [ty] should not be an evar before doing typeclass search *)
+(* [t] should not be an evar before doing typeclass search *)
 Global Hint Mode IntoValTyped - ! - - : typeclass_instances.
 End defs.
