new/golang/defn/core.v
@@ -1,5 +1,4 @@
 (* a set of "core" libraries for goose code, intended to bootstrap models that
 are written in Go and translated with goose *)
 From Perennial.goose_lang Require Export lang notation.
-From New.golang.defn Require Export
-  exception pkg loop list.
+From New.golang.defn Require Export exception pkg loop.
