new/golang/defn/postlang.v
@@ -163,31 +163,27 @@ Inductive is_primitive_zero_val : go.type → ∀ {V} `{!IntoVal V}, V → Prop 
 | is_primitive_zero_val_int16 : is_primitive_zero_val int16 (W16 0)
 | is_primitive_zero_val_int8 : is_primitive_zero_val int8 (W8 0).
 
-End defs.
-End go.
-
-(** [GoContextValid] defines when a GoContext is valid. *)
-Class GoContextValid `{!ffi_syntax} `{!GoContext} :=
+(** [go.ContextValid] defines when a GoContext is valid. *)
+Class ContextValid `{!GoContext} :=
 {
   alloc_underlying t : alloc t = alloc (to_underlying t);
-  alloc_primitive t `{!IntoVal V} (v : V) (H : go.is_primitive_zero_val t v) :
+  alloc_primitive t `{!IntoVal V} (v : V) (H : is_primitive_zero_val t v) :
     alloc t = (λ: <>, ref #v)%V;
   alloc_struct fds : alloc (go.StructType fds) = alloc (go.StructType fds); (* TODO *)
   alloc_array n elem : alloc (go.ArrayType n elem) = alloc (go.ArrayType n elem); (* TODO *)
 
   load_underlying t : load t = load (to_underlying t);
-  load_primitive t (H : go.is_primitive t) : load t = (λ: "l", ! "l")%V;
-  load_struct fds :
-    let body := (foldl (λ '(ld) (fd : go.field_decl),
-                          (ld, let (name, t) := (match fd with
-                                                 | go.FieldDecl n t => (n, t)%core
-                                                 | go.EmbeddedField n t => (n, t)%core
-                                                 end) in
-                               (GoInstruction $ GoLoad t)
-                                 ((GoInstruction $ StructFieldRef (go.StructType fds) name) "l"))%E
-                   ) (Val #()) fds) in
-    load (go.StructType fds) = (λ: "l", body)%V;
+  load_primitive t (H : is_primitive t) : load t = (λ: "l", ! "l")%V;
+  load_struct fds : load (go.StructType fds) = (λ: "l", Panic "impl")%V; (* TODO *)
   load_array n elem : load (go.ArrayType n elem) = load (go.ArrayType n elem); (* TODO *)
+
+  store_underlying t : store t = store (to_underlying t);
+  store_primitive t (H : is_primitive t) : store t = (λ: "l" "v", "l" <- "v")%V;
+  store_struct fds : store (go.StructType fds) = (λ: "l", Panic "impl")%V; (* TODO *)
+  store_array n elem : store (go.ArrayType n elem) = store (go.ArrayType n elem); (* TODO *)
 
   struct_field_ref_underlying t : struct_field_ref t = struct_field_ref (to_underlying t);
 }.
+
+End defs.
+End go.
