new/golang/theory/predeclared.v
@@ -1,0 +1,284 @@
+From New.golang.theory Require Export proofmode.
+From Perennial Require Import base.
+
+Set Default Proof Using "Type".
+
+Section into_val_instances.
+Context `{sem: ffi_semantics} `{!ffi_interp ffi} `{!heapGS Σ} {Hvalid : go.ContextValid}.
+
+Program Global Instance into_val_proof_loc : IntoValProof loc :=
+  {| typed_pointsto_def _ _ _ _ _ _ l dq v := heap_pointsto l dq #v |}.
+Next Obligation. rewrite to_val_unseal => ?? [=] //. Qed.
+
+Program Global Instance into_val_proof_w64 : IntoValProof w64 :=
+  {| typed_pointsto_def _ _ _ _ _ _ l dq v := heap_pointsto l dq #v |}.
+Next Obligation. rewrite to_val_unseal => ?? [=] //. Qed.
+
+Program Global Instance into_val_proof_w32 : IntoValProof w32 :=
+  {| typed_pointsto_def _ _ _ _ _ _ l dq v := heap_pointsto l dq #v |}.
+Next Obligation. rewrite to_val_unseal => ?? [=] //. Qed.
+
+Program Global Instance into_val_proof_w16 : IntoValProof w16 :=
+  {| typed_pointsto_def _ _ _ _ _ _ l dq v := heap_pointsto l dq #v |}.
+Next Obligation. rewrite to_val_unseal => ?? [=] //. Qed.
+
+Program Global Instance into_val_proof_w8 : IntoValProof w8 :=
+  {| typed_pointsto_def _ _ _ _ _ _ l dq v := heap_pointsto l dq #v |}.
+Next Obligation. rewrite to_val_unseal => ?? [=] //. Qed.
+
+Program Global Instance into_val_proof_bool : IntoValProof bool :=
+  {| typed_pointsto_def _ _ _ _ _ _ l dq v := heap_pointsto l dq #v |}.
+Next Obligation. rewrite to_val_unseal => ?? [=] //. Qed.
+
+Program Global Instance into_val_proof_string : IntoValProof go_string :=
+  {| typed_pointsto_def _ _ _ _ _ _ l dq v := heap_pointsto l dq #v |}.
+Next Obligation. rewrite to_val_unseal => ?? [=] //. Qed.
+
+Program Global Instance into_val_proof_slice : IntoValProof slice.t :=
+  {| typed_pointsto_def _ _ _ _ _ _ l dq v := heap_pointsto l dq #v |}.
+Next Obligation. rewrite to_val_unseal => ?? [=] //. Qed.
+
+(* Helper lemmas for establishing [IntoValTyped] *)
+Local Lemma wp_untyped_load l dq v s E :
+  {{{ ▷ heap_pointsto l dq v }}}
+    ! #l @ s; E
+  {{{ RET v; heap_pointsto l dq v }}}.
+Proof. rewrite to_val_unseal. apply lifting.wp_load. Qed.
+
+Local Lemma wp_untyped_store l v v' s E :
+  {{{ ▷ heap_pointsto l (DfracOwn 1) v }}}
+    #l <- v' @ s; E
+  {{{ RET #(); heap_pointsto l (DfracOwn 1) v' }}}.
+Proof.
+  rewrite to_val_unseal. iIntros "% Hl HΦ". wp_call.
+  wp_apply (wp_prepare_write with "Hl"). iIntros "[Hl Hl']".
+  wp_pures. by iApply (wp_finish_store with "[$Hl $Hl']").
+Qed.
+
+Existing Class go.is_primitive.
+#[local] Hint Extern 1 (go.is_primitive ?t) => constructor : typeclass_instances.
+
+Local Ltac solve_wp_load :=
+  iIntros "* Hl HΦ";
+  rewrite go.load_primitive;
+  wp_pures; rewrite typed_pointsto_unseal /=;
+  wp_apply (wp_untyped_load with "Hl");
+  iIntros "Hl"; by iApply "HΦ".
+
+Local Ltac solve_wp_store :=
+  iIntros "* Hl HΦ";
+  rewrite go.store_primitive;
+  wp_pures; rewrite typed_pointsto_unseal /=;
+  wp_apply (wp_untyped_store with "Hl");
+  iIntros "Hl"; by iApply "HΦ".
+
+Local Ltac solve_into_val_typed := constructor; [solve_wp_load|solve_wp_store].
+
+Global Instance into_val_typed_loc t : IntoValTyped loc (go.PointerType t).
+Proof using Hvalid. solve_into_val_typed. Qed.
+
+Global Instance into_val_typed_w64 : IntoValTyped w64 go.uint64.
+Proof using Hvalid. solve_into_val_typed. Qed.
+
+Global Instance into_val_typed_w32 : IntoValTyped w32 go.uint32.
+Proof using Hvalid. solve_into_val_typed. Qed.
+
+Global Instance into_val_typed_w16 : IntoValTyped w16 go.uint16.
+Proof using Hvalid. solve_into_val_typed. Qed.
+
+Global Instance into_val_typed_w8 : IntoValTyped w8 go.uint8.
+Proof using Hvalid. solve_into_val_typed. Qed.
+
+Global Instance into_val_typed_bool : IntoValTyped bool go.bool.
+Proof using Hvalid. solve_into_val_typed. Qed.
+
+Global Instance into_val_typed_string : IntoValTyped go_string go.string.
+Proof using Hvalid. solve_into_val_typed. Qed.
+
+Global Instance into_val_typed_slice t : IntoValTyped slice.t (go.SliceType t).
+Proof using Hvalid. solve_into_val_typed. Qed.
+
+(* Using [vec] here because the [to_val] must be a total function that always
+   meets [has_go_type]. An alternative could be a sigma type. *)
+Program Global Instance into_val_typed_array `{!IntoVal V} `{!IntoValTyped V t} n :
+  IntoValTyped (vec V n) (arrayT n t) :=
+{| default_val := vreplicate n (default_val _) |}.
+Next Obligation.
+  rewrite to_val_unseal /=.
+  solve_has_go_type.
+  induction v as [|].
+  - apply (has_go_type_array 0 t []); done.
+  - simpl in *.
+    inversion IHv. subst.
+    pose proof (has_go_type_array (S (length a)) t (#h::a) ltac:(done)) as Ht.
+    simpl in Ht. apply Ht. intros ? [|].
+    + subst. apply to_val_has_go_type.
+    + apply Helems. done.
+Qed.
+Next Obligation.
+  intros.
+  rewrite to_val_unseal zero_val_eq /=.
+  rewrite -zero_val_unseal -default_val_eq_zero_val.
+  induction n; first done. simpl. f_equal. apply IHn.
+Qed.
+Final Obligation.
+rewrite to_val_unseal.
+intros. intros ?? Heq.
+simpl in Heq.
+induction x.
+{ rewrite (VectorSpec.nil_spec y) //. }
+destruct y using vec_S_inv.
+simpl in *.
+injection Heq as Heq1 Heq.
+apply to_val_inj in Heq1. subst.
+f_equal. by apply IHx.
+Qed.
+
+Program Global Instance into_val_typed_func : IntoValTyped func.t funcT :=
+{| default_val := func.nil |}.
+Next Obligation. solve_has_go_type. Qed.
+Next Obligation. rewrite zero_val_eq //. Qed.
+Next Obligation. rewrite to_val_unseal => [[???] [???]] /= [=] //. naive_solver.
+Qed.
+Final Obligation. solve_decision. Qed.
+
+Program Global Instance into_val_typed_interface : IntoValTyped interface.t interfaceT :=
+{| default_val := interface.nil |}.
+Next Obligation. solve_has_go_type. Qed.
+Next Obligation. rewrite zero_val_eq //. Qed.
+Next Obligation.
+  rewrite to_val_unseal => [x y] Heq.
+  destruct x as [|], y as [|].
+  {
+    simpl in *.
+    injection Heq as Heq1 Heq2.
+    apply to_val_inj in Heq1. subst. done.
+  }
+  all: first [discriminate | reflexivity].
+Qed.
+Final Obligation.
+  solve_decision.
+Qed.
+
+Program Global Instance into_val_typed_unit : IntoValTyped unit (structT []) :=
+{| default_val := tt |}.
+Next Obligation.
+  intros [].
+  replace (#()) with (struct.val_aux (structT []) []).
+  2:{ rewrite struct.val_aux_unseal //. }
+  by constructor.
+Qed.
+Next Obligation. rewrite zero_val_eq /= struct.val_aux_unseal //. Qed.
+Final Obligation.
+  intros ???. destruct x, y. done.
+Qed. *)
+
+End into_val_instances.
+
+
+Section into_val_instances.
+Context `{sem: ffi_semantics} `{!ffi_interp ffi} `{!heapGS Σ}.
+Context `{!NamedUnderlyingTypes}.
+
+Context `{!go.MemOps}.
+Program Global Instance into_val_typed_uint64 : IntoValTyped loc go.uint64.
+Next Obligation.
+  iIntros "* Hl HΦ".
+  rewrite go.load_primitive; [|constructor].
+  wp_pures.
+Admitted.
+Final Obligation. Admitted.
+
+Program Global Instance into_val_typed_loc t : IntoValTyped loc (go.PointerType t).
+Next Obligation.
+  iIntros "* Hl HΦ".
+  rewrite go.load_primitive; [|constructor].
+  wp_pures.
+Admitted.
+Final Obligation. Admitted.
+
+Record foo_t :=
+  mk {
+      a : w64;
+    }.
+Global Instance into_val_foo : IntoVal foo_t :=
+  {| to_val_def := λ v, (#v.(a), #())%V; zero_val := (mk (zero_val _)) |}.
+
+Definition foo_impl : go.type := go.StructType [(go.FieldDecl "a"%go go.uint64)].
+Definition foo : go.type := go.Named "foo"%go [].
+
+Class foo_type_assumptions : Prop :=
+  {
+    foo_underlying : named_to_underlying "foo"%go [] = foo_impl
+  }.
+
+Context `{!foo_type_assumptions}.
+
+(* TODO: struct field_ref. One option is to have field_ref_f be a totally opaque
+   function.  All that really matters is it's a deterministic computation and
+   that it agrees with allocation.
+   E.g. it really doesn't matter if struct fields are packed or not, nor if
+   they're in the same order as source code.
+ *)
+(* TODO: for struct values, what about using a gmap rather than list val?
+   Induction principle might be screwed up. *)
+
+Program Global Instance into_val_proof_w64 : IntoValProof w64 :=
+  {| typed_pointsto_def _ _ _ _ _ _ l dq v := heap_pointsto l dq #v |}.
+Next Obligation. rewrite to_val_unseal => ?? [=] //. Qed.
+
+Program Global Instance into_val_foo_inj : IntoValProof foo_t :=
+  {| typed_pointsto_def _ _ _ _ _ _ l dq v := (struct_field_ref foo "a"%go l ↦{dq} v.(a))%I |}.
+Next Obligation. rewrite to_val_unseal => ?? [=] //. Admitted.
+Next Obligation. solve_decision. Qed.
+
+Lemma foo_split l dq (v : foo_t) :
+  l ↦{dq} v ⊢ (struct_field_ref foo "a"%go l) ↦{dq} v.(a).
+Proof. done. Qed.
+
+Program Global Instance into_val_typed_foo  : IntoValTyped foo_t foo.
+Next Obligation.
+  iIntros "* Hl HΦ".
+  iEval (rewrite go.load_underlying /= foo_underlying go.load_struct /=).
+  wp_pures. wp_bind.
+  iDestruct (foo_split with "Hl") as "Hl".
+  Opaque typed_pointsto. (* FIXME: seal typed_pointsto *)
+  iEval (rewrite go.struct_field_ref_underlying /= foo_underlying /foo_impl) in "Hl".
+  wp_apply (wp_load (t:=go.uint64) with "Hl").
+  iIntros "Hl".
+  wp_pures.
+  (* FIXME: construct StructVal. Have pure op to insert into struct val. Can
+     start from empty struct val. Can give list-like notation. *)
+Admitted.
+
+(* TODO: Maybe aggregate all the built-in dynamic functions into one instruction? *)
+
+Context `{!GoContext}.
+Context `{!MemOps}.
+
+Record foo_t :=
+  mk {
+      a : w64;
+    }.
+Global Instance into_val_foo : IntoVal foo_t :=
+  {| to_val_def := λ v, (#v.(a), #())%V; zero_val := (mk (zero_val _)) |}.
+
+Definition foo : go.type := go.Named "foo"%go [].
+Definition foo_impl : go.type := go.StructType [(go.FieldDecl "a"%go uint64)].
+
+Class foo_type_assumptions : Prop :=
+  {
+    foo_underlying : named_to_underlying "foo"%go [] = foo_impl
+  }.
+
+Context `{!foo_type_assumptions}.
+
+Goal goose_lang.size (go.ArrayType 3 foo) = 3.
+  rewrite size_array size_underlying /= foo_underlying
+    size_struct /= size_primitive //. constructor.
+Qed.
+
+Goal load (go.ArrayType 3 foo) = (λ: "l", ! "l")%V.
+  rewrite is_load_array /=. vm_compute Z.add.
+  rewrite is_load_underlying /= foo_underlying.
+  rewrite is_load_struct /=.
