new/golang/theory/primitive.v
@@ -1,4 +1,4 @@
-From New.golang.theory Require Export typing proofmode.
+From New.golang.theory Require Export proofmode.
 From Perennial Require Import base.
 
 Set Default Proof Using "Type".
