new/golang/theory/slice.v
@@ -3,7 +3,7 @@ From iris.algebra Require Import dfrac.
 From Perennial.iris_lib Require Import dfractional.
 From Perennial.goose_lang Require Import ipersist.
 From New.golang.defn Require Export slice.
-From New.golang.theory Require Import mem list assume exception loop typing auto builtin primitive.
+From New.golang.theory Require Import mem assume exception loop auto builtin primitive.
 From Perennial Require Import base.
 
 Set Default Proof Using "Type".
