new/golang/theory/string.v
@@ -3,14 +3,14 @@ From iris.algebra Require Import dfrac.
 From Perennial.iris_lib Require Import dfractional.
 From Perennial.goose_lang Require Import ipersist.
 From New.golang.defn Require Export string.
-From New.golang.theory Require Import list assume exception loop typing primitive auto.
+From New.golang.theory Require Import assume exception loop primitive auto.
 From New.golang.theory Require Import mem slice.
 From Perennial Require Import base.
 
 Set Default Proof Using "Type".
 
 Section wps.
-  
+
   Context `{hG: heapGS Σ, !ffi_semantics _ _}.
 
   Lemma wp_StringToBytes (s:go_string) :
@@ -19,7 +19,7 @@ Section wps.
   }}}
     string.to_bytes #s
   {{{
-        (sl:slice.t), RET #sl; own_slice sl (DfracOwn 1) s         
+        (sl:slice.t), RET #sl; own_slice sl (DfracOwn 1) s
   }}}.
   Admitted.
 
